

Intertwining operators for \mathfrak{sl}_2 .

Daniil Klyuev

1 Plan and first steps

Let \mathfrak{g} be a simple Lie algebra of rank r , $\mathfrak{b} = \mathfrak{b}_+$ be a Borel subalgebra, \mathfrak{h} be a Cartan subalgebra,

We want to prove that the center $\mathfrak{z}(\hat{\mathfrak{g}})$ of vertex algebra $V_{\kappa_c}(\mathfrak{g})$ at the critical level is isomorphic to $\text{Fun Op}_{G^\vee}(D)$.

In order to do this we will use the homomorphism of vertex algebras

$$\omega_{\kappa_c}: V_{\kappa_c}(\mathfrak{g}) \rightarrow W_{0,\kappa_c} = M_{\mathfrak{g}} \otimes V_0(\mathfrak{h}),$$

constructed in Section 4 of [W] where the notation is as follows: $M_{\mathfrak{g}}$ is the Weyl vertex algebra whose underlying vector space of states is the Fock representation of the Weyl algebra $\mathcal{A}^{\mathfrak{g}}$ and $V_0(\mathfrak{h}) = \pi_0$ is the commutative vertex algebra associated to $L\mathfrak{h}$.

The plan is as follows.

1. Show that ω_{κ_c} is injective.
2. Show that $\omega_{\kappa_c}(\mathfrak{z}(\hat{\mathfrak{g}})) \subset \pi_0$. Hence we need to describe the image of $\mathfrak{z}(\hat{\mathfrak{g}})$ in π_0 .
3. Construct *screening operators* $\overline{S}_i, i = 1, \dots, r$, where r is the rank of \mathfrak{g} , $\hat{\mathfrak{g}}_{\kappa_c}$ -linear maps from W_{0,κ_c} to other modules.
4. Show that $\omega_{\kappa_c}(V_{\kappa_c}(\mathfrak{g})) \subset \ker \overline{S}_i$ for all i . Hence the image of $\mathfrak{z}(\hat{\mathfrak{g}})$ is contained in $\bigcap_{i=1}^l \ker \overline{V}_i[1]$, where $\overline{V}_i[1]$ is the restriction of \overline{S}_i to π_0 .
5. Using the isomorphism between the Wakimoto module $W_{\kappa_c}^+$ and the Verma module \mathbf{M}_{0,κ_c} constructed in Kenta's lecture we will compute the

graded character of $\mathfrak{z}(\hat{\mathfrak{g}})$. We will show that it is equal to the character of $\bigcap_{i=1}^l \ker \overline{V}_i[1]$. It follows that

$$\mathfrak{z}(\hat{\mathfrak{g}}) = \bigcap_{i=1}^l \ker \overline{V}_i[1].$$

6. By using *Miura opers* constructed in Zeyu's talk we will show that there is a natural isomorphism $\mathrm{Fun} \mathrm{Op}_{G^\vee}(D) \cong \bigcap_{i=1}^l \ker \overline{V}_i[1]$. This will yield an isomorphism between $\mathfrak{z}(\hat{\mathfrak{g}})$ and $\mathrm{Fun} \mathrm{Op}_{G^\vee}(D)$. Moreover, all our constructions will be $\mathrm{Aut} \mathcal{O}$ -equivariant.

In my talk I will explain the first and the second steps of this plan, this is relatively quick. I will also explain steps 3-4 for in the case $\mathfrak{g} = \mathfrak{sl}_2$.

1.1 Steps 1 and 2

We want to prove that ω_{κ_c} is injective. First, we discuss a finite-dimensional analogue of this statement.

In Daishi's notes [K] there is a homomorphism of Lie algebras

$$\rho: \mathfrak{g} \rightarrow \mathrm{vect}(B_+)^H = \mathrm{vect}(N_+) \oplus (\mathbb{C}[N_+] \otimes \mathfrak{h}).$$

The right-hand side is contained in $\mathbb{C}[T^*N_+ \times \mathfrak{h}^*]$, so we can extend ρ to

$$\phi^*: \mathbb{C}[\mathfrak{g}^*] \rightarrow \mathbb{C}[T^*N_+ \times \mathfrak{h}^*].$$

Here $\phi: T^*N_+ \times \mathfrak{h}^* \rightarrow \mathfrak{g}^*$ is a morphism of varieties.

We can also extend ρ naturally to

$$\rho: U(\mathfrak{g}) \rightarrow D(N_+) \otimes U(\mathfrak{h}).$$

The map ω_{κ_c} is an affine analog of ρ . Namely, $U(\mathfrak{g})$ corresponds to $V_{\kappa_c}(\mathfrak{g})$, $U(\mathfrak{h})$ corresponds to $V_0(\mathfrak{h})$ and $D(N_+)$, differential operators, corresponds to $M_{\mathfrak{g}}$, that could be realized as chiral differential operators [CDO1].

The injectivity of ρ is proved in Remark 2.4 of [K] as follows: we take the associated graded map of ρ and get $\mathrm{gr} \rho = \phi^*$. After that we show that ϕ is dominant, equivalently, that ϕ^* is injective.

We will use a similar strategy below to prove that ω_{κ_c} is injective. In fact, we will prove a stronger statement:

Proposition 1.1. *The homomorphism $\omega_\kappa: V_\kappa(\mathfrak{g}) \rightarrow M_{\mathfrak{g}} \otimes \pi_0^{\kappa-\kappa_c}$ is injective for any κ .*

Proof. We will introduce filtrations on $V_\kappa(\mathfrak{g})$ and $M_{\mathfrak{g}} \otimes \pi_0^{\kappa-\kappa_c}$ such that ω_κ preserves filtrations and $\text{gr } \omega_\kappa$ is injective. The PBW filtration on $U(\hat{\mathfrak{g}})$ induces a filtration on $V_\kappa(\mathfrak{g})$: $|0\rangle$ has degree zero and x_n with $n < 0$ has degree 1. The filtration on $W_{0,\kappa}$ is defined similarly with $|0\rangle$ in degree 0, and operators $a_{\alpha,n}^*$ with $n \leq 0$ in degree 0 and $a_{\alpha,n}, b_n$ with $n < 0$ in degree 1.

Exercise. 1. T is filtration preserving on each of the vertex algebras.

2. ω_κ is filtration preserving. Hint: look at the formulas in Section 4 of [W] or in Section 1.6 of [CDO2].

3. $\text{gr } \omega_\kappa$ is a homomorphism of graded commutative algebras with differentials.

We know that $\text{gr } V_\kappa(\mathfrak{g}) = \mathbb{C}[J\mathfrak{g}]$ and it can be checked similarly that $\text{gr } W_{0,\kappa} = \mathbb{C}[J(T^*N_+ \times \mathfrak{h}^*)]$. These are the jet schemes of the varieties $\mathfrak{g} \cong \mathfrak{g}^*$, $T^*N_+ \times \mathfrak{h}^*$ considered above.

Exercise. Prove that $\text{gr } \omega_\kappa = (J\phi)^*$, where ϕ is defined above. Hint: for any affine variety X the algebra $\mathbb{C}[JX]$ is graded, the grading is unique such that $\deg T = -1$, $\deg \mathbb{C}[X] = 0$. Here T is the derivation of $\mathbb{C}[JX]$. For a morphism $\varphi: X \rightarrow Y$ the map

$$(J\varphi)^*: \mathbb{C}[JY] \rightarrow \mathbb{C}[JX]$$

is a unique homomorphism such that

1. $(J\varphi)^*$ restricts to $\varphi^*: \mathbb{C}[Y] \rightarrow \mathbb{C}[X]$.

2. $(J\varphi)^*$ intertwines the derivations.

Check that $\text{gr } \omega_\kappa$ satisfies the properties (1) and (2).

It remains to prove that $(J\phi)^*$ is injective. Exercise 2.4 in [K] says that ϕ^* is injective, so that ϕ is dominant. Using Exercise 1.2.13 in Vanya's notes [KL] we get that $J\phi$ is dominant, hence $(J\phi)^*$ is injective. \square

We move to the second step of the plan:

Lemma 1.2. $\omega_{\kappa_c}(\mathfrak{z}(\hat{\mathfrak{g}}))$ is contained in $\pi_0 \subset W_{0,\kappa_c}$.

Proof. We will use the results from Ivan's notes [CDO1, CDO2] that provide an alternative construction of $M_{\mathfrak{g}}$ and ω_{κ_c} using chiral differential operators.

Recall that $\mathfrak{z}(\hat{\mathfrak{g}})$ is the $\mathfrak{g}[[t]]$ -invariants in $V_{\kappa_c}(\mathfrak{g})$. It is enough to prove that

$$\omega_{\kappa_c}(V_{\kappa_c}(\mathfrak{g})^{b+[[t]]}) \subset \pi_0.$$

Note that $V_{\kappa_c}(\mathfrak{g})^{b+[[t]]} = V_{\kappa_c}(\mathfrak{g})^{JB_+}$. The chiral differential operator of realization of W_{0,κ_c} provides a natural action of JB_+ on W_{0,κ_c} , explained in Section 1.2-1.3 of [CDO2]. With this action the map ω_{κ_c} is JB_+ -equivariant, it is an exercise just before section 1.5 of [CDO2].

It follows that

$$\omega_{\kappa_c}(\mathfrak{z}(\hat{\mathfrak{g}})) \subset W_{0,\kappa_c}^{JB_+}.$$

Specializing the results of section 1.5 of [CDO2] to $P_+ = B_+$, $\mathfrak{m} = \mathfrak{h}$, we get

$$\omega_{\kappa_c}(\mathfrak{z}(\hat{\mathfrak{g}})) \subset V_0(\mathfrak{h}) = \pi_0.$$

□

2 Screening operators for \mathfrak{sl}_2

For $\lambda \in \mathbb{C}$ let M_λ, M_λ^* denote, respectively, the Verma and the dual Verma module over \mathfrak{sl}_2 with highest weight λ . We have a short exact sequence

$$0 \rightarrow M_{-2} \rightarrow M_0 \rightarrow L_0 = \mathbb{C} \rightarrow 0,$$

where L_0 is the trivial representation. Applying the duality functor we get a short exact sequence

$$0 \rightarrow \mathbb{C} \rightarrow M_0^* \rightarrow M_{-2}^* \rightarrow 0.$$

We want an affine analogue of this short exact sequence. We will define a homomorphism of $\hat{\mathfrak{sl}}_2$ -modules

$$S_k: W_{0,k} \rightarrow W_{-2,k}$$

for non-critical level k and prove the following

Proposition 2.1. *When $k+2$ is not a nonnegative rational number, we have a short exact sequence*

$$0 \rightarrow V_k(\mathfrak{sl}_2) \rightarrow W_{0,k} \xrightarrow{S_k} W_{-2,k} \rightarrow 0.$$

2.1 Modules over vertex algebras

We will need the notion of a module over a vertex algebra V . This is a vector space M with a map $Y_M: V \rightarrow \text{End}_M[[z^{\pm 1}]]$ such that

1. $Y_M(|0\rangle, z) = \text{Id}_M$
2. For any $u, v \in V$, $m \in M$ the expressions

$$Y_M(u, z)Y_M(v, t)m, \quad Y_M(v, t)Y_M(u, z)m, \quad Y_M(Y(u, z-t)v, t)m$$

are expansions of the same element of $M[[z, t]][z^{-1}, t^{-1}, (z-t)^{-1}]$, similarly to the associativity condition for vertex algebras, [D]

We have the following example. Let $\mathfrak{h} = \mathbb{C}h$ be one-dimensional commutative Lie algebra, so that $\hat{\mathfrak{h}}_\kappa$ is a Heisenberg Lie algebra for nonzero κ and an abelian Lie algebra for $\kappa = 0$. Let $V_\kappa(\mathfrak{h})$ be the corresponding vertex algebra. Consider $M = M_\lambda = \text{Ind}_{\mathfrak{h}[[t]]}^{\hat{\mathfrak{h}}_\kappa} \mathbb{C}_\lambda$, a Verma module over $\hat{\mathfrak{h}}_\kappa$. For $a_1, \dots, a_k < 0$ we define

$$Y_M(h_{a_1}h_{a_2} \cdots h_{a_k}|0\rangle) = \frac{1}{(-a_1-1)! \cdots (-a_k-1)!} \partial_z^{-a_1-1} h(z) \cdots \partial_z^{-a_k-1} h(z) :,$$

similarly to $Y(h_{a_1} \cdots h_{a_k}|0\rangle)$. It can be checked that conditions 1 and 2 are satisfied.

We can upgrade this example. Let $W_{0,k} = M_{\mathfrak{sl}_2} \otimes V_{k+2}(\mathfrak{h})$. Setting $\lambda = -2$ and tensoring by $M_{\mathfrak{sl}_2}$ we get a module $W_{-2,k} = M_{\mathfrak{sl}_2} \otimes \pi_{-2}^{k+2}$ over $W_{0,k}$.

Now we describe basic properties of modules over vertex algebras similar to the associativity and its corollaries for vertex algebras.

If M is a module over V and U is a vertex subalgebra of V , then M is a module over U . In particular, if V is a conformal vertex algebra with central charge c , we get an action of Virasoro vertex algebra Vir_c on M . If $\omega \in V$ is a conformal vector we define endomorphisms L_n^M of M via

$$Y_M(\omega, z) = \sum_{n \in \mathbb{Z}} L_n^M z^{-n-2}.$$

We denote L_{-1}^M by T .

Recall the skew-symmetry property for vertex algebras:

$$Y(A, z)B = e^{zT}Y(B, -z)A.$$

Motivated by this we define a map $Y_{V,M}: M \rightarrow \text{Hom}(V, M)[[z^{\pm 1}]]$ by

$$Y_{V,M}(B, z)A = e^{zT}Y_M(A, -z)B. \quad (1)$$

The following lemma is proved similarly to the associativity property of vertex algebras, [D]:

Lemma 2.2. *For any $A, C \in V$, $B \in M$ there exists an element $f \in M[[z, w]][z^{-1}, w^{-1}, (z - w)^{-1}]$ such that the formal power series*

$$\begin{aligned} Y_M(A, z)Y_{V,M}(B, w)C, & \quad Y_{V,M}(B, w)Y(A, z)C, \\ Y_{V,M}(Y_{V,M}(B, w - z)A, z)C, & \quad Y_{V,M}(Y_M(A, z - w)B, w)C. \end{aligned}$$

are expansions of f in

$$M((z))((w)), \quad M((w))((z)), \quad M((z))((z - w)), \quad M((w))((z - w))$$

respectively.

Abusing the notation, for $A \in V$ we write

$$Y(A, z) = \sum A_{(n)}z^{-n-1}, \quad Y_M(A, z) = A_{(n)}z^{-n-1}.$$

Similarly, for $B \in M$ we write

$$Y_{V,M}(B, w) = \sum B_{(n)}w^{-n-1}.$$

Similarly to the formula for the commutators of fields in vertex algebras [D] we have

$$[B_{(m)}, A_{(k)}] = \sum_{n \geq 0} \binom{m}{n} (B_{(n)}A)_{(m+k-n)}$$

and the same formula with A, B switched:

$$[A_{(m)}, B_{(k)}] = \sum_{n \geq 0} \binom{m}{n} (A_{(n)}B)_{(m+k-n)} \quad (2)$$

It can also be checked that

$$Y_{V,M}(TB, z) = \partial_z Y_{V,M}(B, z). \quad (3)$$

Remark 2.3. Let M be a vector space, V be a vertex algebra. One can show that to give a structure of a module over V on M is the same as to extend a vertex algebra structure from V to $V \oplus M$ such that

1. M is an ideal (this means for any $v \in V$, $m \in M$ and integer i we have $v_{(i)}m \in M$ and $m_{(i)}v \in M$.)
2. For any $m, n \in M$ and integer i we have $m_{(i)}n = 0$.

This is similar to the situation with modules over a commutative algebra: an A -module structure on a vector space M is the same as an algebra structure on $A \oplus M$ such that A is its subalgebra, $AM \subset M$, $M^2 = \{0\}$.

2.2 Definition of S_k and intertwining property

Definition 2.4. The *screening operator* S_k is the residue of

$$Y_{W_{0,k}, W_{-2,k}}(a_{-1}|-2\rangle).$$

We will write an explicit formula for

$$S_k(z) = Y_{W_{0,k}, W_{-2,k}}(a_{-1}|-2\rangle): W_{0,k} \rightarrow W_{-2,k}$$

and prove that $S_k = \text{Res } S_k(z)$ intertwines the action of $\hat{\mathfrak{sl}}_2$.

Lemma 2.5. *We have*

$$S_k(z) = a(z) \otimes \left(T_{-2} \exp \left(\frac{1}{k+2} \sum_{n < 0} \frac{b_n}{n} z^{-n} \right) \exp \left(\frac{1}{k+2} \sum_{n > 0} \frac{b_n}{n} z^{-n} \right) \right), \quad (4)$$

where $T_{-2}: \pi_0^{k+2} \rightarrow \pi_{-2}^{k+2}$ sends $|0\rangle$ to $|-2\rangle$ and commutes with the action of $b_n, n \neq 0$.

Proof. Since $W_{0,k} = M_{\mathfrak{sl}_2} \otimes \pi_0^{k+2}$ and $|-2\rangle_{W_{0,k}} = |0\rangle_{M_{\mathfrak{sl}_2}} \otimes |-2\rangle_{\pi_0^{k+2}}$, we have

$$\begin{aligned} Y_{W_{0,k}, W_{-2,k}}(a_{-1}|-2\rangle) &= Y_{M_{\mathfrak{sl}_2}}(a_{-1}|0\rangle, z) \otimes Y_{\pi_0^{k+2}, \pi_{-2}^{k+2}}(|-2\rangle, z) = \\ &= a(z) \otimes Y_{\pi_0^{k+2}, \pi_{-2}^{k+2}}(|-2\rangle, z). \end{aligned} \quad (5)$$

Let

$$V_{-2}(z) = Y_{\pi_0^{k+2}, \pi_{-2}^{k+2}}(|-2\rangle, z).$$

It remains to compute $V_{-2}(z)$ in order to prove the lemma. We will do this in two steps. First, we will express $V_{-2}(z)$ via $V_{-2}(z)|0\rangle$. Then we will compute $V_{-2}(z)|0\rangle$.

Apply (2) to $A = b_{-1}|0\rangle$, $B = |-2\rangle$ to get

$$[b_m, B_{(k)}] = \sum_{n \geq 0} \binom{m}{n} (b_n |-2\rangle)_{m+k-n} = -2B_{(m+k)},$$

since $b_n |-2\rangle$ is zero for $n > 0$ and $-2|-2\rangle$ for $n = 0$. It follows that

$$[b_m, V_{-2}(z)] = -2z^m V_{-2}(z). \quad (6)$$

Since vectors $b_{n_1} \cdots b_{n_l}|0\rangle$ span π_0^{k+2} , the action of $V_{-2}(z)$ is determined by $V_{-2}(z)|0\rangle \in \pi_{-2}^{k+2}[[z]]$. Namely,

$$V_{-2}(z) = V_{-2}(z)|0\rangle \exp\left(\frac{1}{k+2} \sum_{n>0} \frac{b_n}{n} z^{-n}\right), \quad (7)$$

where $\exp(\frac{1}{k+2} \sum_{n>0} \frac{b_n}{n} z^{-n}) \in \text{End}(\pi_0^k)[[z^{-1}]]$ is a field and $V_{-2}(z)|0\rangle$ is a shorthand for the operator that sends $b_{a_1} \cdots b_{a_k}|0\rangle \in \pi_0^{k+2}$ to

$$b_{a_1} \cdots b_{a_k} V_{-2}(z)|0\rangle \in \pi_{-2}^{k+2}[[z]]$$

for any $a_1, \dots, a_k < 0$. This operator is uniquely defined by the Taylor series $V_{-2}(z)|0\rangle \in \pi_{-2}^{k+2}[[z]]$ that we will compute below.

Now we use equation (3) for $B = |-2\rangle$ to get

$$\partial_z V_{-2}(z) = Y_{V,M}(T|-2\rangle, z).$$

We have the following property of vertex algebras (Corollary 2.3.3 in Frenkel's book or [D]): for any $n, m < 0$ and $A, B \in V$

$$Y(A_{(n)} B_{(m)}, z) = \frac{1}{(-n-1)!(-m-1)!} : \partial_z^{-n-1} Y(A, z) \partial_z^{-m-1} Y(B, z) : .$$

Using Lemma 2.2 for $A = b_{-1}|0\rangle$, $B = |-2\rangle$ and expanding

$$Y_M(A, z) Y_{V,M}(B, w) C = Y_{V,M}(Y_M(A, z-w) B) C$$

in powers of $z-w$ similarly to [D] we get

$$Y_{V,M}(b_{-1}|-2\rangle, z) =: b(z) V_{-2}(z) : .$$

Using Proposition 6.2.2 in Frenkel's book or the third section of [W] we see that the action of $T = L_{-1} = Y(\mathbf{S}_k, z)_{-1}$ on π_0 is given by

$$T = \frac{1}{4(k+2)} \sum_{n \in \mathbb{Z}} b_n b_{-n-1}.$$

Hence

$$-b_{-1}|-2\rangle = (k+2)T|-2\rangle. \quad (8)$$

It follows that

$$(k+2)\partial_z V_{-2}(z) = - : b(z) V_{-2}(z) : . \quad (9)$$

Using (1) for $A = |0\rangle$ we see that for any vertex algebra V , module M over V and $B \in M$ we have

$$Y_{V,M}(B)|0\rangle \in B + zM[[z]] \quad (10)$$

Applying both sides of (9) to $|0\rangle$ we get

$$(k+2)\partial_z(V_{-2}(z)|0\rangle) = -b_+(z)V_{-2}(z)|0\rangle.$$

This is a differential equation for the power series

$$V_{-2}(z)|0\rangle = Y_{\pi_0^{k+2}, \pi_{-2}^{k+2}}(|-2\rangle, z)|0\rangle$$

with constant term $|-2\rangle$, the solution is

$$V_{-2}(z)|0\rangle = \exp\left(\frac{1}{k+2} \sum_{n < 0} \frac{b_n}{n} z^{-n}\right) |-2\rangle.$$

Comparing this with (7) we get

$$V_{-2}(z) = T_{-2} \exp\left(\frac{1}{k+2} \sum_{n < 0} \frac{b_n}{n} z^{-n}\right) \exp\left(\frac{1}{k+2} \sum_{n > 0} \frac{b_n}{n} z^{-n}\right). \quad (11)$$

Using (5) and (7) we get

$$S_k(z) = a(z) \otimes \left(T_{-2} \exp\left(\frac{1}{k+2} \sum_{n < 0} \frac{b_n}{n} z^{-n}\right) \exp\left(\frac{1}{k+2} \sum_{n > 0} \frac{b_n}{n} z^{-n}\right) \right),$$

as claimed. □

Proposition 2.6. *The map S_k is a homomorphism of $\hat{\mathfrak{sl}}_2$ -modules.*

Proof. The plan of the proof is as follows:

1. We will compute the action of $e_n, f_n, h_n, n \geq 0$ on $a_{-1}|-2\rangle$.
2. Using (2) for $A = x_{-1}|0\rangle, B = a_{-1}|-2\rangle$, where $x = e, f, h$, we will show that

$$[A_{(n)}, B_{(0)}] = 0.$$

Since $A_{(n)} = x_n, B_{(0)} = S_k$, this will prove the proposition.

We move to the first step of the plan. Recall that e_n is sent to a_n . Using $\hat{\mathfrak{sl}}_2$ relations we get

$$[e_n, a_{-1}] = 0, \quad [h_n, a_{-1}] = 2a_{n-1}, \quad [f_n, a_{-1}] = -h_{n-1} + k\delta_{n,1}.$$

Recall the formulas for other generators (6.2.3 in Frenkel's book, follows from formulas in section 2 of [W]):

$$h(z) \mapsto -2 : a^*(z)a(z) : + b(z), \quad (12)$$

$$f(z) \mapsto : a^*(z)^2 a(z) : + k\partial_z a^*(z) + a^*(z)b(z). \quad (13)$$

Using these formulas and the grading on the Wakimoto module by degree of t we get

$$e_n|-2\rangle = a_n|-2\rangle = 0, \quad n \geq 0; \quad h_n|-2\rangle = f_n|-2\rangle = 0, \quad n > 0,$$

$$h_0|-2\rangle = -2|-2\rangle.$$

It follows that

$$e_n a_{-1}|-2\rangle = h_n a_{-1}|-2\rangle = 0, \quad n \geq 0.$$

We also have

$$f_n a_{-1}|-2\rangle = 0, \quad n \geq 1; \quad f_1 a_{-1}|-2\rangle = (-h_0 + k)|-2\rangle = (k+2)|-2\rangle. \quad (14)$$

To compute the action of f_0 we have to look more carefully at (13). First we use the $\hat{\mathfrak{sl}}_2$ relation to get

$$f_0 a_{-1}|-2\rangle = a_{-1} f_0|-2\rangle - h_{-1}|-2\rangle.$$

Using (12), (13) and the fact that $a_m|-2\rangle = a_{m+1}^*|-2\rangle = b_{m+1}|-2\rangle = 0$ for $m \geq 0$ we get

$$\begin{aligned} f_0|-2\rangle &= a_0^*b_0|-2\rangle = -2a_0^*|-2\rangle, \\ h_{-1}|-2\rangle &= (-2a_{-1}a_0^* + b_{-1})|-2\rangle. \end{aligned}$$

It follows that

$$f_0a_{-1}|-2\rangle = -b_{-1}|-2\rangle.$$

Using (8) we get

$$f_0a_{-1}|-2\rangle = (k+2)T|-2\rangle. \quad (15)$$

Now we will check that S_k is $\hat{\mathfrak{sl}}_2$ -linear. Set $B = a_{-1}|-2\rangle$ for the computations below. By definition, $S_k = B_{(0)}$.

Using equation (2) for $A = a_{-1}|0\rangle$ we have

$$[A_{(m)}, B_{(k)}] = \sum_{n \geq 0} \binom{m}{n} (A_{(n)}B)_{(m+k-n)} = \sum_{n \geq 0} \binom{m}{n} (a_n a_{-1}|-2\rangle)_{(m+k-n)} = 0.$$

Using (2) for $A = h_{-1}|0\rangle$ we have

$$[A_{(m)}, B_{(k)}] = \sum_{n \geq 0} \binom{m}{n} (A_{(n)}B)_{(m+k-n)} = \sum_{n \geq 0} \binom{m}{n} (h_n a_{-1}|-2\rangle)_{(m+k-n)} = 0.$$

Using (2) for $A = f_{-1}|0\rangle$, $B = a_{-1}|-2\rangle$ we have

$$\begin{aligned} [A_{(m)}, B_{(l)}] &= \sum_{n \geq 0} \binom{m}{n} (A_{(n)}B)_{(m+l-n)} = \sum_{n \geq 0} \binom{m}{n} (f_n a_{-1}|-2\rangle)_{(m+l-n)} \\ &= m(f_1 \cdot a_{-1}|-2\rangle)_{(m+l-1)} + (f_0 \cdot a_{-1}|-2\rangle)_{(m+l)} = (14), (15) \\ &= (k+2)m|-2\rangle_{(m+l-1)} + (k+2)(T|-2\rangle)_{(m+l)} \end{aligned}$$

Now we write

$$\begin{aligned} (T|-2\rangle)_{(m+l)} &= [z^{-1-m-l}]Y(T|-2\rangle, z) \\ &= [z^{-1-m-l}]Y(|-2\rangle, z)' = (-m-l)(|-2\rangle)_{(m+l-1)}. \end{aligned}$$

It follows that

$$[A_{(m)}, B_{(l)}] = -(k+2)l(|-2\rangle)_{(m+l-1)}.$$

In particular, for $l = 0$ we get zero.

We checked that $B_{(0)}$ commutes with the action of e_m, f_m, h_m for all m . Hence $B_{(0)} = \text{Res } S_k(z)$ is an intertwining operator. \square